Util.v
@@ -1,0 +1,48 @@
+
+Require Import List.
+Require Import Coq.Bool.Bool.
+Require Import Coq.Classes.EquivDec.
+
+Fixpoint list_is_set {A : Type} (l : list A) : Prop := 
+  match l with
+  | x :: xs => list_is_set xs /\ ~ In x xs
+  | nil => True
+  end.
+
+(* Some helpers to deal with booleans *)
+
+Lemma beq_true {A : Type} `{EqDec A} (a c : A) :
+  (a ==b c) = true <-> (a === c).
+Proof.
+  unfold equiv_decb; destruct (a == c); firstorder.
+Qed.
+
+Lemma beq_false {A : Type} `{EqDec A} (a b : A) :
+  (a ==b b) = false <-> (a =/= b).
+Proof.
+  unfold equiv_decb; destruct (a == b); firstorder.
+Qed.
+
+Lemma bne_true {A : Type} `{EqDec A} (a c : A) :
+  (a <>b c) = true <-> (a =/= c).
+Proof.
+  unfold nequiv_decb, equiv_decb. rewrite negb_true_iff. destruct (a == c); firstorder.
+Qed.
+
+Lemma bne_false {A : Type} `{EqDec A} (a b : A) :
+  (a <>b b) = false <-> (a === b).
+Proof.
+
+  unfold nequiv_decb, equiv_decb. rewrite negb_false_iff. destruct (a == b); firstorder.
+Qed.
+
+Ltac conv_bool := repeat match goal with
+                         | [ H: context[_ ==b _ = true] |- _ ] => rewrite beq_true in H
+                         | [ H: context[_ ==b _ = false] |- _ ] => rewrite beq_false in H
+                         | [ H: context[_ <>b _ = true] |- _ ] => rewrite bne_true in H
+                         | [ H: context[_ <>b _ = false] |- _ ] => rewrite bne_false in H
+                         | [ H: context[_ || _ = true] |- _ ] => rewrite orb_true_iff in H
+                         | [ H: context[_ || _ = false] |- _ ] => rewrite orb_false_iff in H
+                         | [ H: context[_ && _ = true] |- _ ] => rewrite andb_true_iff in H
+                         | [ H: context[_ && _ = false] |- _ ] => rewrite andb_false_iff in H
+                         end.
